Rename 'step_base' to 'step'
- Most libraries will define their own 'step' relation. Then when we
  create an environment that combines the rules of various 'step'
  relations, we test if the new 'step' relation includes the old 'step'
  relation, and if the sum of the old 'step' relations include the new
  'step' relation.

He4/Discussion/LanguageBase.v
@@ -223,7 +223,7 @@ Proof.
 Reserved Notation "t1 '/' st1 '==>' t2 '/' st2"
   (at level 40, st1 at level 39, t2 at level 39).
 
-Inductive step_base : (prod tm (prod stack store)) -> (prod tm (prod stack store)) -> Prop :=
+Inductive step : (prod tm (prod stack store)) -> (prod tm (prod stack store)) -> Prop :=
   | STnot_r :
     forall t t' st st',
     t / st ==> t' / st' ->
@@ -473,7 +473,7 @@ Inductive step_base : (prod tm (prod stack store)) -> (prod tm (prod stack store
     sr_read n0 sr = tcl c t0 ->
     tfield_w n v0 (tref n0) / pair sk sr ==> tvoid / pair sk (sr_write n0 (tcl c (rc_write n v0 t0)) sr)
 
-  where "t1 '/' st1 '==>' t2 '/' st2" := (step_base (pair t1 st1) (pair t2 st2)).
+  where "t1 '/' st1 '==>' t2 '/' st2" := (step (pair t1 st1) (pair t2 st2)).
 
 Lemma value_does_not_step:
   forall t,
@@ -495,19 +495,19 @@ Proof with auto.
 
 Ltac value_step_impossible :=
   match goal with
-  | H: value ?t, H0: step_base (pair ?t ?st) (pair ?t' ?st') |- _ =>
+  | H: value ?t, H0: step (pair ?t ?st) (pair ?t' ?st') |- _ =>
     solve [destruct (value_does_not_step t H st t' st'); assumption]
   end.
 
-Ltac step_base_impossible :=
+Ltac step_impossible :=
   match goal with
-  | H: step_base _ _ |- _ =>
+  | H: step _ _ |- _ =>
     solve [inversion H]
   end.
 
-Ltac step_base_inductive :=
+Ltac step_inductive :=
   match goal with
-  | H: forall z, step_base ?x z -> z = ?y, H0: step_base ?x ?a |- _ = _ =>
+  | H: forall z, step ?x z -> z = ?y, H0: step ?x ?a |- _ = _ =>
     solve [apply H in H0; inversion H0; auto]
   end.
 
@@ -523,21 +523,21 @@ Ltac equality_contradiction :=
     solve [exfalso; apply H; reflexivity]
   end.
 
-Lemma step_base_deterministic:
+Lemma step_deterministic:
   forall x y,
-  step_base x y ->
+  step x y ->
   forall z,
-    step_base x z ->
+    step x z ->
     z = y.
 Proof with auto.
   intros x y Hxy.
   induction Hxy; intros z Hxz; inversion Hxz; subst;
   try solve [value_step_impossible];
   try solve [auto];
-  try solve [step_base_inductive];
+  try solve [step_inductive];
   try solve [rewrite_invert];
   try solve [equality_contradiction];
-  try solve [step_base_impossible].
+  try solve [step_impossible].
   (* STfield_w_r and STfield_w_l *)
   destruct H5 as [H5 | H5].
   { value_step_impossible. }
